fstar/treesync/code/MLS.TreeSync.API.Types.fst
@@ -9,11 +9,10 @@ open MLS.TreeSync.Invariants.AuthService
 
 (** TreeSync state and accessors *)
 noeq
-type treesync_state (bytes:Type0) {|crypto_bytes bytes|} (tkt:treekem_types bytes) (asp:as_parameters bytes) = {
-  group_id: mls_bytes bytes;
+type treesync_state (bytes:Type0) {|crypto_bytes bytes|} (tkt:treekem_types bytes) (asp:as_parameters bytes) (group_id:mls_bytes bytes) = {
   levels: nat;
   tree: treesync_valid bytes tkt levels 0 group_id;
   tokens: tokens:as_tokens bytes asp.token_t levels 0{all_credentials_ok tree tokens};
 }
 
-type treesync_index (#bytes:Type0) {|crypto_bytes bytes|} (#tkt:treekem_types bytes) (#asp:as_parameters bytes) (st:treesync_state bytes tkt asp) = i:nat{i < pow2 st.levels}
+type treesync_index (#bytes:Type0) {|crypto_bytes bytes|} (#tkt:treekem_types bytes) (#asp:as_parameters bytes) (#group_id:mls_bytes bytes) (st:treesync_state bytes tkt asp group_id) = i:nat{i < pow2 st.levels}
